Machine.v
@@ -1,0 +1,80 @@
+(* Primitive Abstraction. *)
+
+Parameter Word : Type. 
+Parameter wlt : Word -> Word -> bool.
+Parameter weq : Word -> Word -> bool.
+Axiom WordEqDec : forall (w1 w2 : Word), {w1 = w2} + {w1 <> w2}.
+Axiom weq_implies_eq :
+  forall w1 w2,
+    weq w1 w2 = true -> w1 = w2.
+Axiom not_weq_implies_neq :
+  forall w1 w2,
+    weq w1 w2 = false -> w1 <> w2.
+Definition wle (w1 w2: Word) : bool := orb (wlt w1 w2) (weq w1 w2).
+Parameter wplus : Word -> nat -> Word.
+Parameter wminus : Word -> nat -> Word.
+
+Definition Addr : Type := Word.
+
+Parameter Register : Type.
+Parameter PC : Register.
+Parameter SP : Register.
+
+Inductive Component:=
+| Mem (a:Addr)
+| Reg (r:Register).
+
+(* A Value is a Word. *)
+Definition Value : Type := Word.
+
+(* A Machine State is just a map from Components to Values. *)
+Definition MachineState := Component -> Value.
+
+(* Observations are values, or silent (tau) *)
+Inductive Observation : Type := 
+| Out (w:Value) 
+| Tau. 
+
+(* A Machine State can step to a new Machine State plus an Observation. *)
+Parameter step : MachineState -> MachineState * Observation.
+
+Definition CallMap := Value -> nat -> Prop.
+
+Definition isCall (cm: CallMap) (m: MachineState) (args: nat) : Prop :=
+   cm (m (Reg PC)) args.
+
+Definition isRet (mc m: MachineState) : Prop :=
+  m (Reg PC) = wplus (mc (Reg PC)) 4 /\ m (Reg SP) = mc (Reg SP).
+
+Parameter PolicyState : Type.
+Parameter pstep : MachineState * PolicyState -> option PolicyState.
+(* TODO: Does this ever fail? *)
+Parameter initPolicyState : MachineState -> CallMap -> PolicyState.
+
+Definition MPState : Type := MachineState * PolicyState.
+Definition ms (mp : MPState) := fst mp.
+Definition ps (mp : MPState) := snd mp.
+
+Definition mpstep (mp : MPState) :=
+  let (m', O) := step (ms mp) in
+  match pstep mp with
+  | Some p' => Some (m', p', O)
+  | None => None
+  end.
+
+
+(* Confidentiality and Integrity Labels *)
+Inductive CLabel :=
+| HC
+| LC.
+
+Inductive ILabel :=
+| HI
+| LI.
+
+Definition Label := (CLabel * ILabel)%type.
+
+Definition Contour := Component -> Label.
+
+Definition integrityOf (l : Label) : ILabel := snd l.
+Definition confidentialityOf (l : Label) : CLabel := fst l.
